lean/LoVe/LoVe09_OperationalSemantics_ExerciseSheet.lean
@@ -55,16 +55,21 @@ infixr:90 "; " => Stmt.seq
 specification of GCL above. -/
 
 inductive BigStep : (Stmt × State) → State → Prop
-  -- enter the missing `assign` rule here
+  | assign x e s : BigStep (Stmt.assign x e, s) (s[x ↦ e s])
   | assert (B s) (hB : B s) :
     BigStep (Stmt.assert B, s) s
-  -- enter the missing `seq` rule here
+  | seq (C1 C2 s s'' s')
+    (h1: BigStep (C1, s) s'') (h2: BigStep (C2, s'') s'):
+    BigStep (Stmt.seq C1 C2, s) s'
   -- below, `Ss[i]'hless` returns element `i` of `Ss`, which exists thanks to
   -- condition `hless`
   | choice (Ss s t i) (hless : i < List.length Ss)
       (hbody : BigStep (Ss[i]'hless, s) t) :
     BigStep (Stmt.choice Ss, s) t
-  -- enter the missing `loop` rules here
+  | loop_more C s s'' s'
+    (hone: BigStep (C, s) s'') (hloop: BigStep (Stmt.loop C, s'') s'):
+    BigStep (Stmt.loop C, s) s'
+  | loop_stop s : BigStep (Stmt.loop _, s) s
 
 infixl:110 " ⟹ " => BigStep
 
@@ -73,27 +78,101 @@ WHILE language. -/
 
 @[simp] theorem BigStep_assign_iff {x a s t} :
     (Stmt.assign x a, s) ⟹ t ↔ t = s[x ↦ a s] :=
-  sorry
+    by
+      apply Iff.intro
+      {
+        intro h
+        cases h
+        simp
+      }
+      {
+        intro h
+        rw [h]
+        apply BigStep.assign
+      }
 
 @[simp] theorem BigStep_assert {B s t} :
     (Stmt.assert B, s) ⟹ t ↔ t = s ∧ B s :=
-  sorry
+    by
+      apply Iff.intro
+      {
+        intro h
+        cases h
+        simp [hB]
+      }
+      {
+        intro h
+        rw [h.left]
+        apply BigStep.assert
+        apply h.right
+      }
 
 @[simp] theorem BigStep_seq_iff {S₁ S₂ s t} :
     (Stmt.seq S₁ S₂, s) ⟹ t ↔ (∃u, (S₁, s) ⟹ u ∧ (S₂, u) ⟹ t) :=
-  sorry
+    by
+      apply Iff.intro
+      {
+        intro h
+        cases h
+        apply Exists.intro
+        apply And.intro <;> assumption
+      }
+      {
+        intro h
+        cases h
+        apply BigStep.seq _ _ _ w <;> simp [h_1]
+      }
 
 theorem BigStep_loop {S s u} :
     (Stmt.loop S, s) ⟹ u ↔
     (s = u ∨ (∃t, (S, s) ⟹ t ∧ (Stmt.loop S, t) ⟹ u)) :=
-  sorry
+  by
+    apply Iff.intro
+    {
+    intro h
+    cases h with
+    | loop_stop => simp
+    | loop_more =>
+      apply Or.inr
+      apply Exists.intro s''
+      simp [hone, hloop]
+    }
+    {
+      intro h
+      cases h
+      {
+        rw [h_1]
+        apply BigStep.loop_stop
+      }
+      {
+        cases h_1
+        apply BigStep.loop_more _ _ w
+        simp [h]
+        simp [h]
+      }
+    }
 
 /- This one is more difficult: -/
 
 @[simp] theorem BigStep_choice {Ss s t} :
     (Stmt.choice Ss, s) ⟹ t ↔
     (∃(i : ℕ) (hless : i < List.length Ss), (Ss[i]'hless, s) ⟹ t) :=
-  sorry
+  by
+    apply Iff.intro
+    {
+      intro h
+      cases h
+      apply Exists.intro i
+      apply Exists.intro hless
+      assumption
+    }
+    {
+      intro h
+      cases h
+      cases h_1
+      apply BigStep.choice _ _ _ w
+      assumption
+    }
 
 end GCL
 
@@ -104,13 +183,13 @@ def gcl_of : Stmt → GCL.Stmt
   | Stmt.skip =>
     GCL.Stmt.assert (fun _ ↦ True)
   | Stmt.assign x a =>
-    sorry
+    GCL.Stmt.assign x a
   | S; T =>
-    sorry
+    (gcl_of S); (gcl_of T)
   | Stmt.ifThenElse B S T  =>
-    sorry
+    GCL.Stmt.choice [(GCL.Stmt.assert B; gcl_of S), (GCL.Stmt.assert (fun s => ¬(B s)); gcl_of T)]
   | Stmt.whileDo B S =>
-    sorry
+    (GCL.Stmt.loop (GCL.Stmt.assert B; gcl_of S)); (GCL.Stmt.assert (fun s => ¬(B s)))
 
 /- 1.4. In the definition of `gcl_of` above, `skip` is translated to
 `assert (fun _ ↦ True)`. Looking at the big-step semantics of both constructs,
@@ -118,6 +197,7 @@ we can convince ourselves that it makes sense. Can you think of other correct
 ways to define the `skip` case? -/
 
 -- enter your answer here
+-- assign x (fun s => s "x")
 
 
 /- ## Question 2: Program Equivalence
@@ -155,31 +235,110 @@ theorem BigStepEquiv.trans {S₁ S₂ S₃} (h₁₂ : S₁ ~ S₂) (h₂₃ : S
 
 theorem BigStepEquiv.skip_assign_id {x} :
     Stmt.assign x (fun s ↦ s x) ~ Stmt.skip :=
-  sorry
+    by simp [BigStepEquiv]
+
 
 theorem BigStepEquiv.seq_skip_left {S} :
     Stmt.skip; S ~ S :=
-  sorry
+    by simp [BigStepEquiv]
 
 theorem BigStepEquiv.seq_skip_right {S} :
     S; Stmt.skip ~ S :=
-  sorry
+    by simp [BigStepEquiv]
 
 theorem BigStepEquiv.if_seq_while_skip {B S} :
     Stmt.ifThenElse B (S; Stmt.whileDo B S) Stmt.skip ~ Stmt.whileDo B S :=
-  sorry
+    by
+      simp [BigStepEquiv]
+      intro s t
+      apply Iff.intro
+      {
+        intro h
+        cases h
+        simp_all
+        rw [h_1.right]
+        apply BigStep.while_false
+        exact h_1.left
+      }
+      {
+        intro h
+        cases h
+        simp_all
+        apply Exists.intro t_1
+        simp [hbody, hrest]
+        apply Or.inr
+        simp [hcond]
+      }
 
 /- 2.2 (**optional**). Program equivalence can be used to replace subprograms
 by other subprograms with the same semantics. Prove the following so-called
 congruence rules that facilitate such replacement: -/
 
+lemma BigStepEquivE {C1 C2 s s'}
+  (hequiv: C1 ~ C2) (hleft: (C1, s) ⟹  s'):
+  (C2, s) ⟹  s' :=
+  by
+    rw [BigStepEquiv] at hequiv
+    apply (hequiv s s').mp
+    exact hleft
+
 theorem BigStepEquiv.seq_congr {S₁ S₂ T₁ T₂} (hS : S₁ ~ S₂)
       (hT : T₁ ~ T₂) :
     S₁; T₁ ~ S₂; T₂ :=
-  sorry
+    by
+      simp [BigStepEquiv]
+      intro s s'
+      apply Iff.intro
+      {
+        intro h
+        cases h
+        cases h_1
+        apply Exists.intro w
+        apply And.intro
+        apply BigStepEquivE hS left
+        apply BigStepEquivE hT right
+      }
+      {
+        intro h
+        cases h
+        cases h_1
+        apply Exists.intro
+        apply And.intro
+        apply BigStepEquivE (BigStepEquiv.symm hS) left
+        apply BigStepEquivE (BigStepEquiv.symm hT) right
+      }
+
 
 theorem BigStepEquiv.if_congr {B S₁ S₂ T₁ T₂} (hS : S₁ ~ S₂) (hT : T₁ ~ T₂) :
     Stmt.ifThenElse B S₁ T₁ ~ Stmt.ifThenElse B S₂ T₂ :=
-  sorry
+    by
+      simp [BigStepEquiv]
+      intro s s'
+      apply Iff.intro
+      {
+        intro h
+        cases h
+        cases h_1
+        apply Or.inl
+        apply And.intro left
+        apply BigStepEquivE hS right
+        cases h_1
+        apply Or.inr
+        apply And.intro left
+        apply BigStepEquivE hT right
+      }
+      {
+        intro h
+        cases h
+        cases h_1
+        apply Or.inl
+        apply And.intro left
+        apply BigStepEquivE (BigStepEquiv.symm hS) right
+        cases h_1
+        apply Or.inr
+        apply And.intro left
+        apply BigStepEquivE (BigStepEquiv.symm hT) right
+      }
+
 
 end LoVe
